\documentclass[english]{article}

\usepackage{babel}
\usepackage{graphicx}
\usepackage{times}
\usepackage{pifont}
\usepackage[margin=1in]{geometry}
\usepackage{mathtools}
\date{}
\begin{document}




\begin{flushright}
Alexey Tukalo\\
Information Technology,\\
Savonia University of Applied Sciences,\\
Kuopio,\\
Finland,\\
EFA12SF\\
\end{flushright}


\date{\today}



\section{}

$
\begin{rcases}
 H(s)=\frac{ V_o(s)}{V_i (s)}\\
  V_o(s)=\frac{R}{R+\frac{1}{SC}}V_i (s)
\rightarrow \frac{ V_o(s)}{V_i (s)}=\frac{R}{R+\frac{1}{SC}} \quad
\end{rcases}
\rightarrow	H(s)=\frac{R}{R+\frac{1}{SC}} \rightarrow
$\\\\\\\\
$
\rightarrow H(j \Omega)=\frac{R}{R+\frac{1}{j \Omega C}}=\frac{R(R-\frac{1}{j \Omega C})}{R^2+\frac{1}{ (\Omega C)^2}}=\frac{R^2-\frac{R}{j \Omega C}}{R^2+\frac{1}{ (\Omega C)^2}} \rightarrow H(j \Omega)=\frac{R^2-\frac{R}{j \Omega C}}{R^2+\frac{1}{ (\Omega C)^2}}
$\\\\\\\\
$
|H(j \Omega)|=\sqrt{\left(\frac{R^2}{R^2+\frac{1}{(\Omega C)^2}}\right)^2+\left(\frac{\frac{R}{\Omega C}}{R^2+\frac{1}{(\Omega C)^2}}\right)^2} =\sqrt{\frac{R^4+\frac{R^2}{(\Omega C)^2}}{R^2+\frac{1}{(\Omega C)^2}}}=\sqrt{\frac{(\Omega C)^2 R^4+R^2}{(\Omega C)^2} \cdot \frac{(\Omega C)^2}{(R \Omega C)^2+1}}=R
$\\\\\\\\
$
\angle H(j \Omega)=arctg \left( \frac{R^2}{R^2+\frac{1}{(\Omega C)^2}} \cdot \frac{R^2+\frac{1}{(\Omega C)^2}}{\frac{R}{\Omega C}}  \right)= arctg \left( R^2 \cdot \frac{\Omega C}{R}  \right)=arctg(R \Omega C)
$

\section{}
$$
\begin{rcases}
\omega=\Omega T\\
\Omega=2 \pi f \\
T=\frac{1}{F_s}
\end{rcases}
\omega=\frac{2 \pi f}{F_s}
$$
In our case $F_s=1kHz \rightarrow \omega=\frac{2 \pi f}{1kHz}=\frac{\pi f}{500Hz}$\\
a) $f=250Hz \rightarrow \omega=\frac{\pi \cdot 250Hz}{500Hz}=\frac{\pi}{2}$\\
a) $f=500Hz \rightarrow \omega=\frac{\pi \cdot 500Hz}{500Hz}=\pi$\\
a) $f=1kHz \rightarrow \omega=\frac{\pi \cdot 1kHz}{500Hz}=2 \pi$\\

\section{}
$
\begin{rcases}
 H(s)=\frac{ V_o(s)}{V_i (s)}\\
  V_o(s)=\frac{1/SC}{R} V_i(s)
\rightarrow \frac{ V_o(s)}{V_i (s)}=\frac{1}{CRS} \quad
\end{rcases}
\rightarrow	H(s)=\frac{1}{CRS}  \rightarrow
$\\\\\\\\
$
\rightarrow H(j \Omega)=\frac{1}{CRS} =- \frac{j \Omega CR}{(\Omega CR)^2} \rightarrow H(j \Omega)=
- \frac{j \Omega CR}{(\Omega CR)^2}$\\\\\\\\
$
| H(j \Omega)|=\frac{\Omega CR}{(\Omega CR)^2}=\frac{1}{\Omega CR} \rightarrow H(j \Omega)=
\frac{1}{\Omega CR} $\\\\\
The real part is 0 $\rightarrow \angle H(j \Omega)=90^o$

\end{document}
